Halt.v
@@ -1,8 +1,5 @@
 Require Import Arith Function Computation Lia List IMP Util.
 
-Print halts.
-
-
 Definition HALT_0 (f: function) :=
   forall n, f n < 2 /\
   (f n = 1 <-> halts (L_next (nat_to_limp n)) L_initial).
@@ -11,3 +8,75 @@ Definition HALT_0 (f: function) :=
 Definition HALT_ALL (f: function) :=
   forall n, f n < 2 /\
   (f n = 1 <-> forall m, halts (L_next (nat_to_limp n)) (L_input_initial m)).
+
+Definition ENUM_C (f: function) :=
+  (forall n, L_always_halts (nat_to_limp (f n))) /\
+  (forall p: L_prog, L_always_halts p -> exists n, nat_to_limp (f n) = p).
+
+Definition SIM_DIAG (f: function) :=
+  forall n, L_eval (nat_to_limp n) n (f n).
+
+Lemma sim_diag_computable:
+  forall f, HALT_0 f -> turing_computable f ->
+  exists g, turing_computable g /\ SIM_DIAG g.
+Proof.
+Admitted.
+
+Lemma halt_halt_all:
+  forall f, HALT_0 f -> turing_computable f ->
+  exists g, turing_computable g /\ HALT_ALL g.
+Proof.
+Admitted.
+
+Lemma halt_all_enumerate_computable:
+  forall f, HALT_ALL f -> turing_computable f ->
+  exists g, turing_computable g /\ ENUM_C g.
+Proof.
+Admitted.
+
+Lemma composition_computable (f g: function):
+  turing_computable f ->
+  turing_computable g ->
+  turing_computable (fun n => f (g n)).
+Proof.
+Admitted.
+
+Lemma S_computable:
+  turing_computable S.
+Proof.
+Admitted.
+
+Theorem halt_undecidable:
+  forall f, HALT_0 f -> ~turing_computable f.
+Proof.
+  intros. intro.
+  remember (halt_halt_all f H H0) as Hg. clear HeqHg.
+  destruct Hg as [g Hg].
+  destruct Hg.
+
+  remember (sim_diag_computable f H H0) as Hsim. clear HeqHsim.
+  destruct Hsim as [sim Hsim].
+  destruct Hsim as [Hsim Hsim'].
+  clear f H H0.
+
+  remember (halt_all_enumerate_computable g H2 H1) as Hh. clear HeqHh.
+  destruct Hh as [h Hh].
+  destruct Hh.
+  clear g H1 H2.
+  unfold ENUM_C in H0.
+  destruct H0.
+
+  remember (composition_computable S sim S_computable Hsim) as HG. clear HeqHG.
+  destruct HG as [G HG].
+  destruct (nat_to_limp_onto G) as [Gn].
+  unfold evaluates in HG.
+  specialize HG with Gn.
+  unfold SIM_DIAG in Hsim'.
+  specialize Hsim' with Gn.
+  unfold L_eval in Hsim'.
+  rewrite <- H2 in Hsim'.
+  remember (eval_unique (L_next G) (L_input_initial Gn) (sim Gn) (S (sim Gn)) Hsim' HG).
+  lia.
+Qed.
+
+Print Assumptions halt_undecidable.
