IMP.v
@@ -16,8 +16,7 @@ Inductive L_instr :=
   | DIV (rt ra rb: nat)
   | MOD (rt ra rb: nat)
   | EQ (rt ra rb: nat)
-  | JNE (i rc: nat)
-  | JRNE (i rc: nat)
+  | JFNE (i rc: nat)
   | JBNE (i rc: nat)
   | RET (ra: nat)
 .
@@ -31,9 +30,9 @@ Definition L_input_initial (x: nat) := Build_L_state 0 (upd_reg_map empty_reg_ma
 Definition eq (n m: nat) :=
   if Nat.eq_dec n m then 1 else 0.
 
-Definition L_next (p: L_prog) (st: L_state): L_state + nat :=
+Definition L_next' (instr: L_instr) (st: L_state): L_state + nat :=
   let (ip, mem) := st in
-  match nth ip p (RET 0) with
+  match instr with
   | NOP => inl (Build_L_state (ip+1) mem)
   | LDI rt n => inl (Build_L_state (ip+1) (upd_reg_map mem rt n))
   | ADD rt ra rb => inl (Build_L_state (ip+1) (upd_reg_map mem rt (mem ra + mem rb)))
@@ -42,14 +41,41 @@ Definition L_next (p: L_prog) (st: L_state): L_state + nat :=
   | DIV rt ra rb => inl (Build_L_state (ip+1) (upd_reg_map mem rt (mem ra / mem rb)))
   | MOD rt ra rb => inl (Build_L_state (ip+1) (upd_reg_map mem rt (mem ra mod mem rb)))
   | EQ rt ra rb => inl (Build_L_state (ip+1) (upd_reg_map mem rt (eq (mem ra) (mem rb))))
-  | JNE i rc =>
-      inl (Build_L_state (if mem rc then i else ip+1) mem)
-  | JRNE i rc =>
+  | JFNE i rc =>
       inl (Build_L_state (if mem rc then ip+i else ip+1) mem)
   | JBNE i rc =>
       inl (Build_L_state (if mem rc then ip-i else ip+1) mem)
   | RET ra => inr (mem ra)
   end.
 
+Definition L_next (p: L_prog) (st: L_state): L_state + nat :=
+  let (ip, mem) := st in L_next' (nth ip p (RET 0)) st.
 
+Inductive C_instr (P: function -> Prop) :=
+  | LINSTR (instr: L_instr)
+  | CALL (f: function) (prf: P f) (rt ra: nat)
+.
+
+Definition C_prog (P: function -> Prop) := list (C_instr P).
+
+Definition C_next { P: function -> Prop } (p: C_prog P) (st: L_state): L_state + nat :=
+  let (ip, mem) := st in
+  match nth ip p (LINSTR P (RET 0)) with
+  | LINSTR _ instr => L_next' instr st
+  | CALL _ f prf rt ra => inl (Build_L_state (ip+1) (upd_reg_map mem rt (f (mem ra))))
+  end.
+
+Definition L_eval (p: L_prog) (n n': nat) :=
+  eval (L_next p) (L_input_initial n) n'.
+
+Definition turing_computable (f: function) :=
+  exists p: L_prog, evaluates (L_next p) L_input_initial f.
+
+Definition L_always_halts (p: L_prog) := always_halts (L_next p) L_input_initial.
+
+Lemma computable_oracles_computable:
+  forall (f: function) (p: C_prog turing_computable),
+    evaluates (C_next p) L_input_initial f -> turing_computable f.
+Proof.
+Admitted.
 
